meh, contexts and substitution are difficult

tlinks.v
@@ -1,5 +1,9 @@
 (* Set Warnings "-notation-overridden,-parsing". *)
+
+Require Import FunctionalExtensionality.
+Require Import Program.Equality.
 Require Import String.
+
 (* Require Import Coq.Lists.List. Import ListNotations. *)
 
 Inductive K :=
@@ -8,10 +12,12 @@ Inductive K :=
 
 Inductive C :=
 | c_bool : C
+| c_list : C -> C
 with A :=
 | a_t: C -> A
 | a_bool : A
 | a_arrow : A -> A -> A
+| a_list : A -> A
 .
 
 Inductive Constant :=
@@ -24,12 +30,21 @@ Inductive M :=
 | m_var : string -> M
 | m_lam : string -> M -> M
 | m_app : M -> M -> M
+| m_empty : M
 .
 
-Inductive Context :=
-| empty_context : Context
-| bind_term_var : string -> A -> Context -> Context
-.
+Definition Context : Type := string -> option A.
+
+Definition lookup_term_var (G: Context) (x: string) : option A :=
+  G x.
+
+Definition bind_term_var (G: Context) (x: string) (a: A) : Context :=
+  fun y => if string_dec x y then Some a else G x.
+
+(* Inductive Context := *)
+(* | empty_context : Context *)
+(* | bind_term_var : string -> A -> Context -> Context *)
+(* . *)
 
 Definition type_of_constant (c: Constant) : A :=
   match c with
@@ -39,21 +54,23 @@ Definition type_of_constant (c: Constant) : A :=
 
 Inductive type_eq : A -> A -> Prop :=
 | te_bool : type_eq a_bool (a_t c_bool)
+| te_list : forall a b, type_eq a b -> type_eq (a_list a) (a_list b)
 (* | te_symm : forall a b, type_eq a b -> type_eq b a *)
 .
 
-Fixpoint lookup_term_var (Gamma : Context) (v : string) : option A :=
-  match Gamma with
-  | empty_context => None
-  | bind_term_var x x0 x1 => if string_dec x v then Some x0 else lookup_term_var x1 v
-  end.
+(* Fixpoint lookup_term_var (Gamma : Context) (v : string) : option A := *)
+  (* match Gamma with *)
+  (* | empty_context => None *)
+  (* | bind_term_var x x0 x1 => if string_dec x v then Some x0 else lookup_term_var x1 v *)
+  (* end. *)
 
 Inductive has_type : Context -> M -> A -> Prop :=
 | t_c : forall G c, has_type G (m_c c) (type_of_constant c)
 | t_var : forall G v a, lookup_term_var G v = Some a -> has_type G (m_var v) a
-| t_lam : forall G v m a b, has_type (bind_term_var v a G) m b -> has_type G (m_lam v m) (a_arrow a b)
+| t_lam : forall G v m a b, has_type (bind_term_var G v a) m b -> has_type G (m_lam v m) (a_arrow a b)
 | t_app : forall G m n a b, has_type G m (a_arrow a b) -> has_type G n a -> has_type G (m_app m n) b
 | t_ab : forall G m a b, type_eq a b -> has_type G m a -> has_type G m b
+| t_empty : forall G a, has_type G m_empty (a_list a)
 .
 
 Example true_has_type_bool : forall G, has_type G (m_c const_true) a_bool.
@@ -80,6 +97,7 @@ Fixpoint subst (inM : M) (x : string) (withN : M) : M :=
     else m_lam y (subst body x withN)
   | m_app m n =>
     m_app (subst m x withN) (subst n x withN)
+  | m_empty => m_empty
   end.
 
 Notation "m [ x := n ]" := (subst m x n) (at level 90).
@@ -94,11 +112,14 @@ Inductive reduces : M -> M -> Prop :=
 Inductive nf : M -> Prop :=
 | nf_lam : forall x m, nf m -> nf (m_lam x m)
 | nf_bb : forall b, nf_b b -> nf b
+| nf_empty : nf m_empty
 with nf_b : M -> Prop :=
 | nf_app : forall b m, nf_b b -> nf m -> nf_b (m_app b m)
 | nf_c : forall c, nf_b (m_c c)
 | nf_var : forall v, nf_b (m_var v)
 . (* I don't like this at all *)
+
+Definition empty_context := fun (x: string) => @None A.
 
 Lemma progress_empty : forall m a, has_type empty_context m a -> (exists m', reduces m m') \/ nf m.
 Proof.
@@ -126,7 +147,9 @@ Proof.
       * destruct IHhas_type2.
         -- left. destruct H3. exists (m_app m x). constructor. assumption.
         -- right. eauto using nf, nf_b.
+      * inversion H. subst. inversion H2.
   - assumption.
+  - right. auto using nf.
 Qed.
 
 Lemma progress_m : forall G m a, has_type G m a -> (exists m', reduces m m') \/ nf m.
@@ -155,13 +178,37 @@ Proof.
       * destruct IHhas_type2.
         -- left. destruct H3. exists (m_app m x). constructor. assumption.
         -- right. apply nf_bb. constructor. assumption. assumption.
+      * inversion H. subst. inversion H2.
   - assumption. 
+  - auto using nf.
+Qed.
+
+Lemma lookup_bound : forall G v a b, lookup_term_var (bind_term_var G v a) v = Some b -> b = a.
+Proof.
+  intros.
+  unfold lookup_term_var, bind_term_var in H.
+  destruct (string_dec _ _); inversion H; intuition.
 Qed.
 
 Lemma substitution_lemma : forall G x m n a b,
-    has_type (bind_term_var x a G) m b -> has_type G n a -> has_type G (m [x := n]) b.
+    has_type (bind_term_var G x a) m b -> has_type G n a -> has_type G (m [x := n]) b.
 Proof.
   intros.
+  dependent induction H; simpl; eauto using has_type.
+  - simpl in H.
+    destruct (string_dec _ _).
+    + subst. apply lookup_bound in H. subst. assumption.
+    + eauto using has_type. apply t_var.
+      (* Uh, do I need that x is unbound in G? That's not easy with
+      the functional representation. Ugh. This is why people don't
+      want to do substitution themselves... *) 
+  - destruct (string_dec _ _).
+    + admit.
+    + simpl.
+      constructor.
+      eapply IHhas_type.
+      (* Crap. This is not true. I think I need to change my contexts.
+      I need to be able to reshuffle them. *)
 Admitted.
 
 Lemma preservation_m : forall G m n a, has_type G m a -> reduces m n -> has_type G n a.
@@ -183,4 +230,5 @@ Proof.
     + eauto using t_app.
     + eauto using t_app.
   - eauto using t_ab.
+  - inversion 1.
 Qed.
